\documentclass{amsart}
\usepackage{ctex}
\begin{document}

设 $x=1+t$,
\begin{align*}
	\frac{\ln(1+x)}{x}&
	=\frac{\ln(2+t)}{1+t}
	=\frac{\ln 2+\ln(1+t/2)}{1+t}\\
	&=\bigl(\ln 2+\frac t2-\frac{t^2}8+o(t^3)\bigr)\bigl(1-t+t^2+o(t^3)\bigr)\\
	&=\ln2+(\frac12-\ln 2)t+(\ln 2-\frac 58)t^2+o(t^3),\\
	x\bigl(\ln(1+x)-\ln x\bigr)&
	=(1+t)(\ln 2+\ln(1+\frac t2)-\ln(1+t))\\
	&=(1+t)\bigl(\ln 2-\frac t2+\frac 38 t^2+o(t^3)\bigr)\\
	&=\ln 2+(\ln 2-\frac 12)t-\frac 18t^2+o(t^3),\\
	S=\frac{\ln(1+x)}{x}+x\ln(1+\frac 1x)
	&=\ln 4+(\ln 2-\frac 34)t^2+o(t^3),\\
	(1+x)^{1/x}(1+\frac1x)^x-4
	&=e^S-4
	=4(\ln 2-\frac 34)t^2+o(t^3),
\end{align*}
故
\[\lim_{x\to 1}\frac{(1+x)^{1/x}(1+\frac1x)^x-4}{(x-1)^2}=4\ln 2-3.\]

\end{document}