\documentclass[handout,aspectratio=169]{ctexbeamer}
\usepackage{animate}
\usepackage{graphicx}


\usepackage{upgreek}

% \newcommand{\skewmathbb}[2]{\scalebox{1}[1]{\skew{#1}{\mathbb{#2}}}}
% \newcommand{\bbsl}[1]{\skewmathbb{2.5}{#1}}

\DeclareSymbolFont{lettersA}{U}{txmia}{m}{it}
\DeclareMathSymbol{\alphaup}{\mathord}{lettersA}{11}
\DeclareMathSymbol{\betaup}{\mathord}{lettersA}{12}
\NewDocumentCommand{\bdgrk}{m m}{
	#1\hspace{#2}#1\hspace{#2}#1\hspace{#2}#1\hspace{#2}#1\hspace{#2}#1
}
\NewDocumentCommand{\bdalpha}{}{\bdgrk{$\alphaup$}{-6.35pt}}
\NewDocumentCommand{\bdbeta}{}{\bdgrk{$\betaup$}{-5.75pt}}

% \def\cstsl#1#2{%
%   \tikz[baseline=(X.base), xslant=tan(#1)]
%     \node[inner sep=0pt, xslant=tan(#1)](X){#2};%
% }
% \newcommand{\slbbH}{\text{\cstsl{10}{$\mathbb{H}$}}}
% \newcommand{\slbbD}{\text{\cstsl{10}{$\mathbb{D}$}}}

\newcommand\boldgreekalpha{
  \tikz{
	\foreach \i in {0,0.003,0.006,...,0.015}{
    \draw (\i,0) node[inner sep=0pt] {$\alphaup$};}
	}
}


\input{../cn_teach}
\title{复变函数与积分变换}

\begin{document}
\begin{frame}{卷积的性质}\small
	\onslide<+->
	\begin{proof}[nearprev]
		\bigdel\bigdel
		\begin{align*}
			\msf[f_1\ast f_2]&=\intff \intff f_1(\tau)f_2(t-\tau)\d \tau \cdot \ee^{-\ii \omega t}\d t\\
			&\visible<+->{=\intff \intff f_1(\tau)\ee^{-\ii \omega \tau}\cdot f_2(t-\tau)\ee^{-\ii \omega (t-\tau)}\d t\d \tau}\\
			&\visible<+->{=\intff \intff f_1(\tau)\ee^{-\ii \omega \tau}\cdot f_2(t)\ee^{-\ii \omega t}\d t\d \tau}\\
			&\visible<+->{=\intff f_1(\tau)\ee^{-\ii \omega \tau}\d\tau\intff f_2(t)\ee^{-\ii \omega t}\d t}\visible<+->{=\msf[f_1]\msf[f_2].\qedhere}
		\end{align*}
	\end{proof}
	\onslide<+->
	由函数的乘法性质可知卷积满足如下性质:
	\begin{itemize}\bf
		\item $f_1\ast f_2=f_2\ast f_1,\ (f_1\ast f_2)\ast f_3=f_1\ast(f_2\ast f_3)$;
		\item $f_1\ast(f_2+f_3)=f_1\ast f_2+f_1\ast f_3$;
		\item $f\ast\dirac=f$;
		\item $(f_1\ast f_2)'=f_1'\ast f_2=f_1\ast f_2'$.
	\end{itemize}
\end{frame}



\end{document}